theories/FOL/Reductions/H10p_to_FA.v
@@ -1,7 +1,7 @@
 From Undecidability.FOL.Util Require Import Syntax Syntax_facts FullTarski FullDeduction_facts FullDeduction FA_facts.
 Require Import Undecidability.FOL.PA.
 From Undecidability.H10 Require Import H10p.
-
+Require Import List.
 
 
 Fixpoint embed_poly p : term :=
@@ -60,20 +60,103 @@ Proof.
 Qed.
 
 
-(* Lemma prv_poly sigma q Gamma : *)
-(*   FA <<= Gamma -> Gamma ⊢I ( (embed_poly q)[sigma >> num] == num (dp_eval sigma q) ). *)
-(* Proof. *)
-(*   intros H. *)
-(*   induction q; cbn. *)
-(*   - change ((num n)[sigma >> num]) with (subst_term (sigma >> num) (num n)). *)
-(*     rewrite numeral_subst_invariance. *)
-(*     now apply reflexivity. *)
-(*   - now apply reflexivity. *)
-(*   - destruct d; cbn. *)
-(*     + eapply transitivity. assumption. *)
-(*       apply (eq_add _ _ H IHq1 IHq2). *)
-(*       now apply num_add_homomorphism. *)
-(*     + eapply transitivity. assumption. *)
-(*       apply (eq_mult _ _ H IHq1 IHq2). *)
-(*       now apply num_mult_homomorphism. *)
-(* Qed. *)
+Lemma prv_poly sigma q Gamma :
+  incl FA_facts.FA Gamma -> Gamma ⊢I ( (embed_poly q)`[sigma >> num] == num (dp_eval_pfree sigma q) ).
+Proof.
+  intros H.
+  induction q; cbn.
+  - change ((num n)`[sigma >> num]) with (subst_term (sigma >> num) (num n)).
+    rewrite numeral_subst_invariance.
+    now apply reflexivity.
+  - now apply reflexivity.
+  - destruct d; cbn.
+    + eapply transitivity. assumption. 
+      apply (eq_add _ _ H IHq1 IHq2).
+      now apply num_add_homomorphism.
+    + eapply transitivity. assumption.
+      apply (eq_mult _ _ H IHq1 IHq2).
+      now apply num_mult_homomorphism.
+Qed.
+
+
+
+Lemma problem_to_prv :
+  forall E sigma, H10p_sem E sigma -> FA_facts.FA ⊢I (embed_problem E)[sigma >> num].
+Proof.
+  intros [a b] sigma HE. cbn -[FA].
+  eapply transitivity; firstorder.
+  apply prv_poly; firstorder.
+  apply symmetry; firstorder.
+  unfold H10p_sem in *. cbn in HE. rewrite HE.
+  apply prv_poly; firstorder.
+Qed.
+
+
+
+  Section FA_Model.
+
+    Context {D : Type}.
+    Context {I : interp D}.
+
+    Hypothesis ext_model : extensional I.
+    Hypothesis FA_model : forall rho ax, In ax FA -> rho ⊨ ax.
+    
+
+    Fact eval_num sigma n : eval sigma (num n) = iμ n.
+    Proof.
+      induction n.
+      - reflexivity.
+      - cbn. now rewrite IHn.
+    Qed.
+    
+    Lemma problem_to_model E sigma : H10_sem E sigma -> (sigma >> iμ) ⊨ embed_problem E.
+    Proof.
+      intros HE%problem_to_prv%Soundness.
+      specialize (HE D I).
+      setoid_rewrite sat_comp in HE.
+      eapply sat_ext. 2: apply HE.
+      intros x. unfold ">>". now rewrite eval_num.
+      intros. instantiate (1 := (fun _ => iO)). now apply sat_FA.  
+    Qed.
+    
+    
+  End FA_Model.
+
+
+
+
+Theorem Reduction_sat :
+  forall E, H10p_SAT E <-> valid_ctx FA_facts.FA (embed E).
+Proof.
+  split.
+  - intros [sigma HE].
+    intros D I rho H.
+    eapply subst_exist_sat.
+    apply problem_to_model.
+    + intros ρ' ax Hax. eapply sat_closed.
+      2: now apply H.
+      repeat (destruct Hax as [<- | Hax]; auto).
+    + apply HE.
+    + rewrite <-exists_close_form; apply embed_is_closed.
+  - intros H.
+    specialize (H nat interp_nat id (nat_is_FA_model id)).
+    unfold embed in *. apply subst_exist_sat2 in H.
+    destruct H as [sigma Hs]. exists sigma.
+    now apply nat_sat.
+Qed.
+
+
+
+Theorem Reduction_prv : forall E, H10p_SAT E <-> FA_facts.FA ⊢I embed E.
+Proof.
+  intros E. split.
+  - intros [sigma HE].
+    eapply subst_exist_prv.
+    apply problem_to_prv,  HE.
+    rewrite <-exists_close_form; apply embed_is_closed.
+  - intros H%soundness.
+    (* now apply Reduction_sat. *)
+Admitted.
+
+
+
